make.sh
@@ -1,0 +1,3 @@
+#!/bin/bash
+coq_makefile -R "." Cat -o makefile *v Limits/*v OldLimits/*v Instances/*v Instances/*/*v
+make
